elo-coq/Map.v
@@ -1,102 +1,120 @@
 From Coq Require Import Strings.String.
-From Coq Require Import Lists.List.
 
-Local Definition map' (A : Type) := string -> A. (* total map *)
+Inductive map (A : Type) : Type :=
+  | nil
+  | cons (k : string) (v : A) (m : map A)
+  .
 
-Local Definition empty' {A : Type} v : map' A := (fun _ => v).
+Definition empty {A} := nil A.
 
-Local Definition update' {A : Type} (m : map' A) k v :=
-  fun k' => if String.eqb k k' then v else m k'.
+Fixpoint update {A} (m : map A) k v :=
+  match m with
+  | nil _ => cons A k v (nil A)
+  | cons _ k' v' m' =>
+      if eqb k k'
+        then cons A k  v  (update m' k v)
+        else cons A k' v' (update m' k v)
+  end.
 
-Definition map (A : Type) := map' (option A). (* partial map *)
+Local Definition update' {A} m k v := cons A k v m.
 
-Definition empty {A : Type} : map A := empty' None.
+Fixpoint lookup {A} m k : option A :=
+  match m with
+  | nil _ => None
+  | cons _ k' v m' => if eqb k' k then Some v else lookup m' k
+  end.
 
-Definition update {A : Type} (m : map A) k v :=
-  update' m k (Some v).
-
-Definition lookup {A : Type} (m : map A) k := m k.
-
-(* Proofs *)
-
-Local Lemma lookup_update_involutive' : forall {A} (m : map A) k v,
-  (update m k v) k = Some v.
+Theorem update_equivalence : forall {A} (m : map A) k v id,
+  lookup (update m k v) id = lookup (update' m k v) id.
 Proof.
-  intros.
-  unfold update, Map.update'.
-  rewrite String.eqb_refl.
-  reflexivity.
+  intros *. unfold update', update.
+  induction m as [| k' v' m IH]; trivial.
+  unfold lookup in *.
+  destruct (eqb k k') eqn:E1.
+  - apply eqb_eq in E1. subst. destruct (eqb k' id); trivial.
+  - destruct (eqb k' id) eqn:E2; trivial.
+    apply eqb_eq in E2. subst.
+    destruct (eqb k id) eqn:E3; trivial; discriminate.
 Qed.
 
-(* TODO : names *)
-Lemma lookup_update_involutive : forall {A} (m : map A) k v,
+Corollary update_equivalence_impl : forall {A} (m : map A) k k' v v',
+  lookup (update m k' v') k = Some v <-> lookup (update' m k' v') k = Some v.
+Proof.
+  intros *. rewrite update_equivalence. split; trivial.
+Qed.
+
+Lemma lookup_update_k_eq : forall {A} (m : map A) k v,
   lookup (update m k v) k = Some v.
 Proof.
-  unfold lookup. intros.
-  apply lookup_update_involutive'.
+  intros. rewrite update_equivalence.
+  simpl. rewrite String.eqb_refl. reflexivity.
 Qed.
 
-(* TODO : names *)
-Lemma lookup_update_idempotent : forall {A} (m : map A) k k' v,
+Lemma lookup_update_k_neq : forall {A} (m : map A) k k' v,
   k' <> k ->
   lookup (update m k' v) k = lookup m k.
 Proof.
-  intros * H.
-  unfold lookup, update, update'.
-  destruct (String.eqb k' k) eqn:E.
-  - apply String.eqb_eq in E. contradiction.
-  - reflexivity.
+  intros * H. rewrite update_equivalence.
+  simpl. destruct eqb eqn:E; trivial.
+  apply String.eqb_eq in E. contradiction.
 Qed.
 
 (* m includes m' *)
-Definition includes' {A} (m m' : map A) := forall k v,
-  m' k = Some v -> m k = Some v.
+Local Definition includes_definition {A} (m m' : map A) :=
+  forall k v, lookup m' k = Some v -> lookup m k = Some v.
 
-Infix "includes" := includes' (at level 50, left associativity).
+Infix "includes" := includes_definition (at level 50, left associativity).
 
 Lemma update_preserves_inclusion : forall {A} (m m' : map A) k v,
   m includes m' ->
   (update m k v) includes (update m' k v).
 Proof.
-  unfold includes'.
-  intros * H k' v' H'.
-  unfold update, update' in *.
-  destruct (String.eqb k k') eqn:E.
-  - assumption.
-  - specialize (H k' v'). auto.
+  intros * ? k' ? H.
+  unfold includes_definition in *. 
+  rewrite update_equivalence in *.
+  unfold lookup, update' in *.
+  destruct m; destruct (eqb k k'); eauto.
+Qed.
+
+Lemma update_overwrite : forall {A} (m : map A) k v v',
+  (update m k v) includes (update (update m k v') k v).
+Proof.
+  intros *. unfold includes_definition. intros k' ?.
+  rewrite 2 update_equivalence.
+  unfold lookup, update'.
+  destruct m; intros H; destruct (eqb k k') eqn:E; trivial;
+  rewrite update_equivalence in H;
+  unfold lookup, update' in H;
+  rewrite E in H; assumption.
 Qed.
 
 Lemma update_permutation : forall {A} (m : map A) k1 k2 v1 v2,
   k1 <> k2 ->
-  update (update m k1 v1) k2 v2 includes update (update m k2 v2) k1 v1.
+  (update' (update' m k1 v1) k2 v2) includes (update' (update' m k2 v2) k1 v1).
 Proof.
-  unfold includes'. intros * H k v.
-  unfold update, update'.
-  destruct (String.eqb k1 k) eqn:E1;
-  destruct (String.eqb k2 k) eqn:E2;
-  auto.
-  apply String.eqb_eq in E1, E2. subst. contradiction.
-Qed.
-
-Lemma update_overwrite : forall {A} (m : map A) k v v',
-  update m k v includes update (update m k v') k v.
-Proof.
-  intros * k' m'.
-  unfold update, update'.
-  destruct (String.eqb k k') eqn:E1; intros; assumption.
-Qed.
-
-(* unused *)
-Lemma update_empty : forall {A} k1 k2 (v1 v2 : A),
-  k1 <> k2 ->
-  update (update empty k1 v1) k2 v2 includes (update empty k1 v1).
-Proof.
-  intros * Hneq.
-  unfold includes'. intros k v.
-  unfold update, Map.update'.
-  destruct (String.eqb k1 k) eqn:E1, (String.eqb k2 k) eqn:E2.
-  - apply String.eqb_eq in E1, E2. subst. contradiction.
-  - trivial.
-  - unfold empty, Map.empty'. intros F. inversion F.
-  - unfold empty, Map.empty'. intros F. inversion F.
+  intros * Hneq. unfold includes_definition.
+  induction m as [| ? ? ? IH]; intros k' v'.
+  - unfold update', lookup.
+    destruct (eqb k1 k') eqn:E1; trivial.
+    destruct (eqb k2 k') eqn:E2; trivial.
+    apply eqb_eq in E1. apply eqb_eq in E2. subst.
+    contradiction.
+  - specialize (IH k' v').
+    destruct (eqb k1 k') eqn:E1.
+    + apply eqb_eq in E1. subst.
+      destruct (eqb k2 k') eqn:E2.
+      * apply eqb_eq in E2. subst. rewrite 2 lookup_update_k_eq in *. trivial.
+      * apply eqb_neq in E2.
+        rewrite (lookup_update_k_neq _ _ _ _ E2).
+        rewrite 2 lookup_update_k_eq in *.
+        intros H. specialize (IH H).
+        assumption.
+    + apply eqb_neq in E1.
+      rewrite (lookup_update_k_neq _ _ _ _ E1) in *.
+      destruct (eqb k2 k') eqn:E2.
+      * apply eqb_eq in E2. subst. rewrite 2 lookup_update_k_eq. trivial.
+      * apply eqb_neq in E2.
+        rewrite 2 (lookup_update_k_neq _ _ _ _ E2) in *.
+        rewrite (lookup_update_k_neq _ _ _ _ E1) in *.
+        trivial.
 Qed.
