elo-coq/Safety.v
@@ -1,0 +1,32 @@
+From Coq Require Import Init.Nat.
+
+From Elo Require Export Core.
+
+Definition synchronize (threads : list tm) (i j : nat) : Prop := False.
+
+Definition happens_before (threads : list tm) i j : Prop :=
+  if i =? j then i < j else synchronize threads i j.
+
+Definition is_write (t : tm) : Prop := 
+  match t with
+  | TM_Asg _ _ | TM_ArrAsg _ _ _ => True
+  | _ => False
+  end.
+
+Definition data_race := forall (threads : list tm) i j,
+  (is_write (get_tm threads i) \/ is_write (get_tm threads j)) /\
+  ~ happens_before threads i j.
+
+(*
+Inductive happens_before' : mem -> tm -> mem -> tm -> Prop :=
+  | HB_Step : forall m m' t t',
+    m / t -->* m' / t' ->
+    happens_before' m t m' t'
+  .
+*)
+
+(*
+  Invariant:
+    At any time during program execution, each thread or monitor can only
+    access memory locations that are either local or safe.
+*)
